Frame.v
@@ -1,0 +1,94 @@
+(* This file is part of the LLIR Semantics project. *)
+(* Licensing information is available in the LICENSE file. *)
+(* (C) 2020 Nandor Licker. All rights reserved. *)
+
+Require Import Coq.Lists.List.
+Require Import Coq.ZArith.ZArith.
+Require Import Coq.Init.Nat.
+
+Require Import LLIR.Maps.
+Require Import LLIR.Values.
+Require Import LLIR.LLIR.
+Require Import LLIR.Dom.
+Require Import LLIR.Liveness.
+Require Import LLIR.Typing.
+
+
+Import ListNotations.
+
+
+
+Record object := mkdata
+  { dt_size: positive
+  ; dt_align: positive
+  ; dt_data: PTrie.t quad
+  }.
+
+Definition objects := PTrie.t object.
+
+Record frame := mkframe
+  { fr_data: objects
+  ; fr_regs: PTrie.t value
+  ; fr_args: list value
+  ; fr_func: name
+  ; fr_pc: node
+  }.
+
+Definition frame_map := PTrie.t frame.
+
+Record stack := mkstack
+  { stk_fr: positive
+  ; stk_frs: list positive
+  ; stk_frames: PTrie.t frame
+  ; stk_init: objects
+  }.
+
+Inductive TopFrame: stack -> Prop :=
+  | top_frame:
+    forall
+      (frames: PTrie.t frame) (init: objects) (top: positive),
+      TopFrame (mkstack top [] frames init)
+  .
+
+Inductive ReturnFrame: stack -> positive -> list positive -> Prop :=
+  | return_frame:
+    forall 
+      (frames: PTrie.t frame) (init: objects) (top: positive) (ret: positive)
+      (frs: list positive),
+      ReturnFrame (mkstack top (ret :: frs) frames init) ret frs
+  .
+
+Lemma top_or_return:
+  forall (stk: stack),
+    TopFrame stk 
+    \/
+    exists (next: positive) (rest: list positive), 
+      ReturnFrame stk next rest.
+Proof.
+  intros stk; destruct stk as [stk_fr' stk_frs' stk_frames' stk_init'].
+  destruct stk_frs'.
+  - left; constructor.
+  - right; exists p; exists stk_frs'; constructor.
+Qed.
+
+Inductive ValidFrame: prog -> frame -> Prop :=
+  | valid_frame:
+    forall
+      (p: prog) (fr: frame)
+      (fr_id: positive) (frames: PTrie.t frame)
+      (data: objects) (args: PTrie.t value)
+      (f: func) (i: inst)
+      (FUNC: Some f = p ! (fr.(fr_func)))
+      (REACH: Reachable f (fr.(fr_pc)))
+      (INST: Some i = f.(fn_insts) ! (fr.(fr_pc)))
+      (REGS:
+        forall (r: reg),
+          LiveAt f r (fr.(fr_pc)) ->
+          exists (v: value),
+            Some v = fr.(fr_regs) ! r)
+      (VALS:
+        forall (r: reg) (v: value),
+          Some v = fr.(fr_regs) ! r ->
+            exists (t: ty), Some t = (ty_env f) ! r /\ TypeOfValue v t),
+      ValidFrame p fr
+  .
