State.v
@@ -1,0 +1,59 @@
+(* This file is part of the LLIR Semantics project. *)
+(* Licensing information is available in the LICENSE file. *)
+(* (C) 2020 Nandor Licker. All rights reserved. *)
+
+Require Import Coq.Lists.List.
+Require Import Coq.ZArith.ZArith.
+
+Require Import LLIR.LLIR.
+Require Import LLIR.Maps.
+Require Import LLIR.Typing.
+Require Import LLIR.Frame.
+
+Import ListNotations.
+
+Record heap := mkheap
+  { hp_segments: PTrie.t objects
+  }.
+
+Record state := mkstate
+  { st_stack: stack
+  ; st_heap: heap
+  }.
+
+
+Definition trace := list (positive * list value).
+
+Inductive ValidTopFrame : prog -> positive -> frame_map -> Prop :=
+  | valid_top_frame:
+    forall
+      (p: prog) (fr_id: positive) (frames: frame_map) (fr: frame)
+      (FRAME: Some fr = frames ! fr_id)
+      (VALID: ValidFrame p fr),
+      ValidTopFrame p fr_id frames
+  .
+
+Inductive ValidMidFrame : prog -> positive -> frame_map -> Prop :=
+  | valid_mid_frame:
+    forall
+      (p: prog) (fr_id: positive) (frames: frame_map) (fr: frame) 
+      (i: inst) (f: func)
+      (FRAME: Some fr = frames ! fr_id)
+      (VALID: ValidFrame p fr)
+      (FUNC: Some f = p ! (fr.(fr_func)))
+      (EXEC: Some i = f.(fn_insts) ! (fr.(fr_pc)))
+      (RETURN: VoidCallSite i \/ (exists (t: ty) (dst: reg), CallSite i t dst)),
+      ValidMidFrame p fr_id frames
+  .
+
+Inductive ValidState : prog -> state -> Prop :=
+  | valid_state:
+    forall
+      (p: prog)
+      (fr_id: positive) (frs: list positive) (frames: PTrie.t frame) (init: objects)
+      (h: heap)
+      (FR: ValidTopFrame p fr_id frames)
+      (NEXT: forall (fr: positive), In fr frs -> ValidMidFrame p fr frames),
+      ValidState p (mkstate (mkstack fr_id frs frames init) h)
+  .
+
